@prefix : <https://rdf.equinor.com/completion#> .
@prefix imf: <http://ns.imfid.org/imf#> .
@prefix owl: <http://www.w3.org/2002/07/owl#> .
@prefix rdf: <http://www.w3.org/1999/02/22-rdf-syntax-ns#> .
@prefix xsd: <http://www.w3.org/2001/XMLSchema#> .
@prefix comp: <https://rdf.equinor.com/completion#> .
@prefix rdfs: <http://www.w3.org/2000/01/rdf-schema#> .
@prefix dexpi: <https://rdf.equinor.com/dexpi#> .
@base <https://rdf.equinor.com/completion#> .

<https://rdf.equinor.com/completion> rdf:type owl:Ontology ;
                                      owl:imports <https://rdf.equinor.com/dexpi> ;
                                      rdfs:comment "Temporary toy ontology for boundaries and completion packages in Dexpi" .

#################################################################
#    Object Properties
#################################################################

###  https://rdf.equinor.com/completion#isBoundaryOf
comp:isBoundaryOf rdf:type owl:ObjectProperty ;
                  rdfs:domain dexpi:PipingOrEquipment ;
                  rdfs:range comp:CompletionPackage ;
                  rdfs:comment "This relates an object in a P&ID to a completion package that it is part of the boundary for. This relation is usually entered manually by engineers and used for the calculation of the completion package." ;
                  rdfs:label "is boundary of" .


###  https://rdf.equinor.com/completion#isInPackage
comp:isInPackage rdf:type owl:ObjectProperty ;
                 rdfs:domain dexpi:PipingOrEquipment ;
                 rdfs:range dexpi:PipingOrEquipment ;
                 rdfs:comment "This relates something in a P&ID to a completion package that it is in. Usually this relation is calculated from the boundary and rules in the ontology" ;
                 rdfs:label "is in completion package" .
#################################################################
#    Classes
#################################################################

###  https://rdf.equinor.com/completion#CompletionPackage
comp:CompletionPackage rdf:type owl:Class ;
                       rdfs:comment "Completion packages are groups of equipment that need to be handled together. The group is usually defined implicitly by defining the boundary." ;
                       rdfs:label "Completion package" .


###  Generated by the OWL API (version 4.5.26.2023-07-17T20:34:13Z) https://github.com/owlcs/owlapi
